title change and responses

lean/src/basic.lean
@@ -71,6 +71,8 @@ def based_on_frame {α: Type} (m : Model α) (f : Frame α) :=
   ∀ aa : set (set α), (∀ a ∈ aa, exp a) -> exp (⋂₀ aa)
 @[simp] def closed_under_unions {α : Type} (exp : set α -> Prop) :=
   ∀ aa : set (set α), (∀ a ∈ aa, exp a) -> exp (⋃₀ aa)
+@[simp] def closed_under_finite_intersections {α : Type} (exp : set α -> Prop) :=
+  exp set.univ ∧ ∀ a b : set α, exp a -> exp b -> exp (a ∩ b)
 @[simp] def closed_under_compl {α : Type} (exp : set α -> Prop) :=
   ∀ a : set α, exp a -> exp aᶜ
 
@@ -85,6 +87,60 @@ def based_on_frame {α: Type} (m : Model α) (f : Frame α) :=
   closed_under_unions m.has_expertise
 @[simp] def mclosed_under_compl {α : Type} (m : Model α) :=
   closed_under_compl m.has_expertise
+
+-- closure under intersections implies closure under finite intersections
+lemma int_implies_finite_int {α : Type} (exp : set α -> Prop) :
+  closed_under_intersections exp -> closed_under_finite_intersections exp :=
+begin
+  intros h,
+  apply and.intro,
+    rw <-set.sInter_empty,
+    apply h ∅,
+    intros,
+    apply absurd (set.not_mem_empty a),
+    simp,
+    assumption,
+
+    intros a b h_a_exp h_b_exp,
+    rw <-set.sInter_pair,
+    apply h {a, b},
+    intros c hmem,
+    apply or.elim (set.eq_or_mem_of_mem_insert hmem),
+      intro h_c_eq_a,
+      rw h_c_eq_a,
+      assumption,
+
+      simp,
+      intro h_c_eq_b,
+      rw h_c_eq_b,
+      assumption,
+end
+
+lemma finset_intersections {α : Type} (exp : set α -> Prop) :
+  closed_under_finite_intersections exp ->
+    ∀ aa : finset (set α), (∀ a ∈ aa, exp a) -> exp (⋂₀ aa) :=
+begin
+  intros h_cl_fin_int aa,
+  apply finset.cons_induction_on aa,
+    -- case a = ∅
+    intros,
+    simp,
+    exact h_cl_fin_int.left,
+
+    -- inductive step
+    intros b aa h_b_not_mem_aa ih h,
+    simp,
+    apply h_cl_fin_int.right,
+      apply h b,
+      simp,
+
+      apply ih,
+      intros,
+      apply h,
+      simp,
+      apply or.inr,
+      assumption,
+end
 
 -- misc
 
